HOL-Light/x86_64: Add proof for poly_decompress_d5
Signed-off-by: Hanno Becker <beckphan@amazon.co.uk>

proofs/hol_light/common/mlkem_specs.ml
@@ -435,6 +435,32 @@ let IVAL_DECOMPRESS_D4_BOUND = prove
   REWRITE_TAC[INT_OF_NUM_LE; INT_OF_NUM_LT; LE_0] THEN ASM_ARITH_TAC);;
 
 (* ------------------------------------------------------------------------- *)
+(* decompress_d5 computes round(u * 3329 / 32)                               *)
+(* which equals (u * 3329 + 16) >> 5 for u in 0..31.                         *)
+(* This is Decompress_5 from FIPS 203, Eq (4.8).                             *)
+(* ------------------------------------------------------------------------- *)
+let decompress_d5 = new_definition
+  `decompress_d5 (x:5 word) : 16 word =
+   word((val x * 3329 + 16) DIV 32)`;;
+
+let IVAL_DECOMPRESS_D5_BOUND = prove
+ (`!x:5 word. &0 <= ival(decompress_d5 x) /\ ival(decompress_d5 x) < &3329`,
+  GEN_TAC THEN
+  SUBGOAL_THEN `val(decompress_d5 (x:5 word)) < 2 EXP 15` ASSUME_TAC THENL
+  [REWRITE_TAC[decompress_d5; VAL_WORD; DIMINDEX_16] THEN
+   MP_TAC(ISPEC `x:5 word` VAL_BOUND) THEN CONV_TAC(DEPTH_CONV DIMINDEX_CONV) THEN ARITH_TAC;
+   ALL_TAC] THEN
+  SUBGOAL_THEN `val(decompress_d5 (x:5 word)) < 3329` ASSUME_TAC THENL
+  [REWRITE_TAC[decompress_d5; VAL_WORD; DIMINDEX_16] THEN
+   MP_TAC(ISPEC `x:5 word` VAL_BOUND) THEN CONV_TAC(DEPTH_CONV DIMINDEX_CONV) THEN ARITH_TAC;
+   ALL_TAC] THEN
+  MP_TAC(ISPEC `decompress_d5 (x:5 word):16 word` IVAL_EQ_VAL) THEN
+  REWRITE_TAC[DIMINDEX_16; ARITH] THEN ASM_REWRITE_TAC[] THEN
+  ANTS_TAC THENL [ASM_ARITH_TAC; ALL_TAC] THEN
+  DISCH_THEN SUBST1_TAC THEN
+  REWRITE_TAC[INT_OF_NUM_LE; INT_OF_NUM_LT; LE_0] THEN ASM_ARITH_TAC);;
+
+(* ------------------------------------------------------------------------- *)
 (* From |- (x == y) (mod m) /\ P   to   |- (x == y) (mod n) /\ P             *)
 (* ------------------------------------------------------------------------- *)
 
@@ -1141,3 +1167,181 @@ let VAL_WORD_EXACT = prove(
 let VAL_WORD_ZX_EXACT = prove(
   `!(x:M word). val x < 2 EXP dimindex(:N) ==> val(word_zx x : N word) = val x`,
   REWRITE_TAC[VAL_WORD_ZX_GEN] THEN SIMP_TAC[MOD_LT]);;
+
+let WORD_SUBWORD_NUM_OF_WORDLIST = prove
+ (`!(ls:(L word)list) k.
+    dimindex(:KL) = dimindex(:L) * LENGTH ls /\
+    k < LENGTH ls
+    ==> word_subword (word (num_of_wordlist ls) : KL word) (dimindex(:L)*k, dimindex(:L)) : L word = EL k ls`,
+  REPEAT STRIP_TAC THEN REWRITE_TAC[GSYM VAL_EQ; VAL_WORD_SUBWORD] THEN
+  REWRITE_TAC[ARITH_RULE `MIN n n = n`] THEN
+  SUBGOAL_THEN `val (word (num_of_wordlist (ls:(L word)list)) : KL word) = num_of_wordlist ls` SUBST1_TAC THENL
+  [W(MP_TAC o PART_MATCH (lhand o rand) VAL_WORD_EQ o lhand o snd) THEN
+   ANTS_TAC THENL
+   [TRANS_TAC LTE_TRANS `2 EXP (dimindex(:L) * LENGTH (ls:(L word)list))` THEN
+    REWRITE_TAC[NUM_OF_WORDLIST_BOUND; LE_EXP; LE_REFL] THEN ASM_ARITH_TAC;
+    SIMP_TAC[]];
+   MP_TAC(ISPECL [`ls:(L word)list`; `k:num`] NUM_OF_WORDLIST_EL) THEN
+   ASM_REWRITE_TAC[]]);;
+
+(* ------------------------------------------------------------------------- *)
+(* Some list lemmas, likely of more general use                              *)
+(* ------------------------------------------------------------------------- *)
+
+(* Flatten a list of lists *)
+let NUM_OF_WORDLIST_FLATTEN = prove
+ (`!(ll:((N word) list) list) k.
+     ALL (\l. LENGTH l = k) ll /\
+     dimindex(:N) * k = dimindex(:M)
+     ==> num_of_wordlist (ITLIST APPEND ll []) =
+         num_of_wordlist (MAP ((word:num->M word) o num_of_wordlist) ll)`,
+  LIST_INDUCT_TAC THEN REWRITE_TAC[ITLIST; MAP; num_of_wordlist; ALL] THEN
+  X_GEN_TAC `k:num` THEN STRIP_TAC THEN
+  FIRST_X_ASSUM(MP_TAC o SPEC `k:num`) THEN
+  ASM_REWRITE_TAC[] THEN DISCH_TAC THEN
+  REWRITE_TAC[NUM_OF_WORDLIST_APPEND; num_of_wordlist; o_THM] THEN
+  ASM_REWRITE_TAC[] THEN
+  AP_THM_TAC THEN AP_TERM_TAC THEN
+  IMP_REWRITE_TAC [VAL_WORD_EXACT] THEN
+  TRANS_TAC LTE_TRANS `2 EXP (dimindex(:N) * LENGTH(h:(N word)list))` THEN
+  REWRITE_TAC[NUM_OF_WORDLIST_BOUND_LENGTH] THEN
+  ASM_REWRITE_TAC[LE_REFL]);;
+
+let EL_SUB_LIST = prove(
+ `!l:'a list. !i k n. i < n /\ k + n <= LENGTH l
+   ==> EL i (SUB_LIST (k, n) l) = EL (k + i) l`,
+  LIST_INDUCT_TAC THENL [
+    REWRITE_TAC[LENGTH; LE; ADD_EQ_0] THEN ARITH_TAC;
+    REWRITE_TAC[LENGTH] THEN REPEAT GEN_TAC THEN
+    STRUCT_CASES_TAC (SPEC `k:num` num_CASES) THEN
+    STRUCT_CASES_TAC (SPEC `n:num` num_CASES) THEN
+    REWRITE_TAC[LT; SUB_LIST_CLAUSES; ADD_CLAUSES] THENL [
+      STRUCT_CASES_TAC (SPEC `i:num` num_CASES) THEN
+      REWRITE_TAC[EL; HD; TL; ADD_CLAUSES] THEN STRIP_TAC THEN
+      FIRST_X_ASSUM (MP_TAC o SPECL [`n:num`; `0`; `n':num`]) THEN
+      REWRITE_TAC[ADD_CLAUSES] THEN DISCH_THEN MATCH_MP_TAC THEN ASM_ARITH_TAC;
+      REWRITE_TAC[EL; TL] THEN STRIP_TAC THEN
+      FIRST_X_ASSUM (MP_TAC o SPECL [`i:num`; `n':num`; `SUC n''`]) THEN
+      ASM_REWRITE_TAC[LT_SUC] THEN DISCH_THEN MATCH_MP_TAC THEN ASM_ARITH_TAC]]);;
+
+(* EL_SUB_LIST_CONV: Rewrites EL i (SUB_LIST (base,len) ls) to EL (base+i) ls
+   Takes a LENGTH ls = n theorem and checks i < len before applying. *)
+let EL_SUB_LIST_CONV len_thm tm =
+  (* Parse EL i (SUB_LIST (base,len) ls) *)
+  let i_tm,sublist_tm = dest_comb tm in
+  let el_const,i = dest_comb i_tm in
+  let sublist_pair,ls = dest_comb sublist_tm in
+  let sublist_const,pair_tm = dest_comb sublist_pair in
+  let base,len = dest_pair pair_tm in
+  (* Check i < len *)
+  let i_num = dest_numeral i and
+      len_num = dest_numeral len in
+  if i_num >= len_num then failwith "EL_SUB_LIST_CONV: index out of bounds" else
+  (* Apply EL_SUB_LIST theorem and simplify *)
+  let th1 = ISPECL [ls; i; base; len] EL_SUB_LIST in
+  let th2 = REWRITE_RULE[len_thm] th1 in
+  let th3 = MP th2 (EQT_ELIM(NUM_REDUCE_CONV (fst(dest_imp(concl th2))))) in
+  (* Evaluate base + i *)
+  CONV_RULE (RAND_CONV (LAND_CONV NUM_ADD_CONV)) th3;;
+
+(* Derived from LENGTH_SUB_LIST *)
+let LENGTH_SUB_LIST_0 = prove
+ (`!n (l:'a list). n <= LENGTH l ==> LENGTH (SUB_LIST (0, n) l) = n`,
+  REPEAT STRIP_TAC THEN REWRITE_TAC[LENGTH_SUB_LIST; SUB_0] THEN ASM_ARITH_TAC);;
+
+let SUB_LIST_SUB_LIST_0 = prove(
+ `!k n m (l:'a list). k + n <= m /\ m <= LENGTH l
+   ==> SUB_LIST (k, n) (SUB_LIST (0, m) l) = SUB_LIST (k, n) l`,
+  REPEAT STRIP_TAC THEN REWRITE_TAC[LIST_EQ; LENGTH_SUB_LIST; SUB_0] THEN
+  CONJ_TAC THENL [ASM_ARITH_TAC; ALL_TAC] THEN REPEAT STRIP_TAC THEN
+  SUBGOAL_THEN `n' < n` ASSUME_TAC THENL [ASM_ARITH_TAC; ALL_TAC] THEN
+  MP_TAC (ISPECL [`SUB_LIST (0,m) l:'a list`; `n':num`; `k:num`; `n:num`] EL_SUB_LIST) THEN
+  MP_TAC (ISPECL [`l:'a list`; `n':num`; `k:num`; `n:num`] EL_SUB_LIST) THEN
+  ASM_REWRITE_TAC[LENGTH_SUB_LIST; SUB_0] THEN
+  SUBGOAL_THEN `k + n <= LENGTH (l:'a list)` ASSUME_TAC THENL [ASM_ARITH_TAC; ALL_TAC] THEN
+  SUBGOAL_THEN `k + n <= MIN m (LENGTH (l:'a list))` ASSUME_TAC THENL [ASM_ARITH_TAC; ALL_TAC] THEN
+  ASM_SIMP_TAC[] THEN REPEAT DISCH_TAC THEN
+  MP_TAC (ISPECL [`l:'a list`; `k + n':num`; `0`; `m:num`] EL_SUB_LIST) THEN
+  ASM_REWRITE_TAC[ADD_CLAUSES] THEN DISCH_THEN MATCH_MP_TAC THEN ASM_ARITH_TAC);;  
+
+(* Variant of SUB_LIST_TOPSPLIT with equality hypothesis *)
+let SUB_LIST_SPLIT_EQ = prove
+ (`!n r (l:'a list). n + r = LENGTH l
+   ==> APPEND (SUB_LIST (0, n) l) (SUB_LIST (n, r) l) = l`,
+  REPEAT STRIP_TAC THEN
+  MP_TAC (ISPECL [`l:'a list`; `n:num`] SUB_LIST_TOPSPLIT) THEN
+  FIRST_X_ASSUM (SUBST1_TAC o SYM) THEN REWRITE_TAC[ADD_SUB2]);;
+
+let APPEND_ITLIST_APPEND_NIL = prove
+ (`!(l:('a list) list) (x:'a list). APPEND (ITLIST APPEND l []) x = ITLIST APPEND l x`,
+  LIST_INDUCT_TAC THEN REWRITE_TAC[ITLIST; APPEND] THEN
+  GEN_TAC THEN REWRITE_TAC[GSYM APPEND_ASSOC] THEN ASM_REWRITE_TAC[]);;
+
+let LIST_OF_SEQ_EQ = prove
+ (`!(f:num->'a) g n. (!i. i < n ==> f i = g i) ==> list_of_seq f n = list_of_seq g n`,
+  GEN_TAC THEN GEN_TAC THEN INDUCT_TAC THEN REWRITE_TAC[list_of_seq] THEN
+  DISCH_TAC THEN BINOP_TAC THENL [
+    FIRST_X_ASSUM MATCH_MP_TAC THEN GEN_TAC THEN DISCH_TAC THEN
+    FIRST_X_ASSUM MATCH_MP_TAC THEN ASM_ARITH_TAC;
+    REWRITE_TAC[CONS_11] THEN FIRST_X_ASSUM MATCH_MP_TAC THEN ARITH_TAC
+  ]);;
+
+let SUBLIST_PARTITION = prove
+ (`!r s (l:'a list). LENGTH l = r * s ==>
+       l = ITLIST APPEND (list_of_seq (\i. SUB_LIST (r * i, r) l) s) []`,
+  GEN_TAC THEN INDUCT_TAC THENL [
+    REWRITE_TAC[MULT_CLAUSES; list_of_seq; ITLIST; LENGTH_EQ_NIL];
+
+    REWRITE_TAC[list_of_seq; ITLIST_EXTRA; APPEND_NIL] THEN
+    GEN_TAC THEN DISCH_TAC THEN
+    SUBGOAL_THEN
+      `SUB_LIST (0, r * s) l =
+       ITLIST APPEND (list_of_seq (\i. SUB_LIST (r * i, r) (SUB_LIST (0, r * s) l)) s) []:'a list`
+      ASSUME_TAC THENL [
+      FIRST_X_ASSUM MATCH_MP_TAC THEN
+      MATCH_MP_TAC LENGTH_SUB_LIST_0 THEN ASM_ARITH_TAC;
+      ALL_TAC
+    ] THEN
+    SUBGOAL_THEN
+      `list_of_seq (\i. SUB_LIST (r * i, r) (SUB_LIST (0, r * s) l):'a list) s =
+       list_of_seq (\i. SUB_LIST (r * i, r) l) s`
+      ASSUME_TAC THENL [
+      MATCH_MP_TAC LIST_OF_SEQ_EQ THEN REPEAT STRIP_TAC THEN REWRITE_TAC[] THEN
+      MATCH_MP_TAC SUB_LIST_SUB_LIST_0 THEN CONJ_TAC THENL [
+        REWRITE_TAC[ARITH_RULE `r * i + r = r * (i + 1)`] THEN
+        REWRITE_TAC[LE_MULT_LCANCEL] THEN ASM_ARITH_TAC;
+        ASM_ARITH_TAC
+      ];
+      ALL_TAC
+    ] THEN
+    SUBGOAL_THEN
+      `APPEND (SUB_LIST (0, r * s) l) (SUB_LIST (r * s, r) l) = l:'a list`
+      ASSUME_TAC THENL [
+      MATCH_MP_TAC SUB_LIST_SPLIT_EQ THEN ASM_REWRITE_TAC[MULT_SUC] THEN ARITH_TAC;
+      ALL_TAC
+    ] THEN
+    SUBGOAL_THEN
+      `SUB_LIST (0, r * s) l =
+       ITLIST APPEND (list_of_seq (\i. SUB_LIST (r * i, r) l) s) []:'a list`
+      ASSUME_TAC THENL [ASM_MESON_TAC[]; ALL_TAC] THEN
+    UNDISCH_TAC `APPEND (SUB_LIST (0,r * s) l) (SUB_LIST (r * s,r) l) = l:'a list` THEN
+    UNDISCH_TAC `SUB_LIST (0,r * s) l = ITLIST APPEND (list_of_seq (\i. SUB_LIST (r * i,r) l) s) []:'a list` THEN
+    SIMP_TAC[APPEND_ITLIST_APPEND_NIL]
+  ]);;
+
+let NUM_BIT_DECOMPOSE_UNIQ = prove(`!a b t k. a < 2 EXP k ==> (a + 2 EXP k * b = t <=> (a = t MOD 2 EXP k /\ b = t DIV 2 EXP k))`,
+    REPEAT STRIP_TAC THEN EQ_TAC THENL [
+      DISCH_THEN (SUBST1_TAC o SYM) THEN
+      SIMP_TAC[MOD_MULT_ADD; DIV_MULT_ADD; EXP_EQ_0; ARITH_EQ] THEN
+      ASM_SIMP_TAC[MOD_LT; DIV_LT; ADD_CLAUSES];
+      STRIP_TAC THEN
+      MP_TAC (SPECL [`t:num`; `2 EXP k`] DIVISION) THEN
+      SIMP_TAC[EXP_EQ_0; ARITH_EQ] THEN ASM_REWRITE_TAC[] THEN ARITH_TAC]);;  
+
+let READ_BYTES_SPLIT_ANY =  prove(`read (bytes(a : int64,k+l)) s = t <=> 
+         read (bytes(a,k)) s = t MOD 2 EXP (8*k) /\ read (bytes(word_add a (word k), l)) s = t DIV 2 EXP (8*k)`,
+      let bound = prove(`read (bytes (a : int64,k)) s < 2 EXP (8*k)`, REWRITE_TAC[READ_BYTES_BOUND]) in
+      REWRITE_TAC[GSYM VAL_EQ; VAL_READ_WBYTES; READ_COMPONENT_COMPOSE] THEN         
+      REWRITE_TAC [READ_BYTES_COMBINE] THEN
+      REWRITE_TAC [MATCH_MP NUM_BIT_DECOMPOSE_UNIQ bound]
+  );;
